\documentclass[journal,12pt,twocolumn]{IEEEtran}
\usepackage{amsmath,amsfonts,amssymb,float,gvv,graphicx,enumitem,array}
\bibliographystyle{IEEEtran}
\vspace{3cm}
\title{NCERT Discrete}
\author{Pragnidhved Reddy\\EE23BTECH11050}
\date{}
\parindent 0px
\begin{document}
\maketitle
\newpage
\bigskip
\textbf{Question 11.9.3.18:}\\
 Find the sum to n terms of the sequence $8,88,888,8888$\ldots\\
 \solution
\begin{table}[H]
\centering
\setlength{\extrarowheight}{8pt}
\begin{tabular}{|c|c|c|}\hline
\textbf{Parameter} & \textbf{Value} & \textbf{description}\\ \hline
$x(0)$ & 8 & First term \\ \hline
$x(1)$ & 88 & Second term \\ \hline 
$x(n)$ & $(\sum^{n}_{k=0}8(10)^k)u(n)$ & General term \\ \hline
$S(n)$ & $S(n)=\sum^{n-1}_{k=0}x(k)$ & Sum of n terms \\ \hline
\end{tabular}
\caption{Input parameters}
\label{tab:table1}
\end{table}
\begin{enumerate}
 \item From \eqref{tab:table1}
\begin{align}
\label{eq:1}
 S(n)&=\sum^{n-1}_{l=0}(\sum^{l}_{k=0}8(10)^k)u(l)
 \end{align}
 \item On solving \eqref{eq:1}, we get
 \begin{align}
 \implies S(n)&=\left(\frac{8}{81}\right)(10^{n+1}-9n-10)
 \end{align}
 \item Z transform of general term
 \begin{align}
 X(z)&=\sum_{l=-\infty}^{\infty}(\sum_{k=0}^{l}8(10)^k)u(n)z^{-l}\\[6pt]
 X(z)&=\sum_{l=0}^{\infty}(\sum_{k=0}^{l}8(10)^k)z^{-l}\\[6pt]
 \implies X(z)&=\frac{8}{9}\left(\frac{100z^{-1}}{1-10z^{-1}}-\frac{z^{-1}}{1-z^{-1}}\right) \quad \abs{z}>10
 \end{align}
 \end{enumerate}
 \end{document}
